\documentclass[dvipdfmx,autodetect-engine,titlepage]{jsarticle}
\usepackage[dvipdfm]{graphicx}
\usepackage{ascmac}
\usepackage{fancybox}
\usepackage{listings}
\usepackage{plistings}
\usepackage{itembkbx}
\usepackage{amsmath}
\usepackage{amssymb}
\usepackage{amsfonts}
\usepackage{svg}
\usepackage{url}
\usepackage{graphics}
\usepackage{multirow}
\usepackage{listings,jvlisting}

\textheight=23cm
\renewcommand{\figurename}{図}
\renewcommand{\tablename}{表}
\newenvironment{code}
{\vspace{0.5zw}\VerbatimEnvironment  
\begin{screen} 
\baselineskip=1.0\normalbaselineskip
 \begin{Verbatim}}
{\end{Verbatim}
\baselineskip=\normalbaselineskip
 \end{screen}\vspace{0.5zw}} 

\title{情報理工学部　SNコース 3回\\
第一回レポート(分散と共分散)\\}
\author{2600200443-6\\Yamashita Kyohei\\山下 恭平}
\date{Jun 23 2022}

\begin{document}

\maketitle

\section{}

以下の式を証明する。

\begin{align*}
  Cov(x+y,z) &= Cov(x,z) + Cov(y,z)\\
\end{align*}

右辺より

\begin{align*}
Cov(x,z) + Cov(y,z) &= \frac{1}{n}\sum (x_{n}-\bar{x})(z_{n}-\bar{z}) + \frac{1}{n}\sum (y_{n}-\bar{y})(z_{n}-\bar{z})\\
&= \frac{1}{n}\sum (x_{n}-\bar{x}+y_{n}-\bar{y})(z_{n}-\bar{z})\\
&= \frac{1}{n}\sum \{ (x_{n}+y_{n})-(\bar{x}+\bar{y})\} (z_{n}-\bar{z})\\
&= Cov(x+y,z) = 左辺
\end{align*}


\end{document}